theories/case_studies/vae/vae_helper.v
@@ -1,0 +1,319 @@
+From iris.proofmode Require Import proofmode.
+From cap_machine Require Import region_invariants_allocation region_invariants_revocation interp_weakening monotone.
+
+Section VAE_helper.
+  Context
+    {Σ:gFunctors}
+    {ceriseg:ceriseG Σ} {sealsg: sealStoreG Σ}
+    {Cname : CmptNameG}
+    {stsg : STSG Addr region_type Σ} {heapg : heapGS Σ}
+    {nainv: logrel_na_invs Σ}
+    {cstackg : CSTACKG Σ}
+    `{MP: MachineParameters}
+    {swlayout : switcherLayout}
+  .
+
+  Context {C : CmptName}.
+
+  Implicit Types W : WORLD.
+  Implicit Types C : CmptName.
+  Notation V := (WORLD -n> (leibnizO CmptName) -n> (leibnizO Word) -n> iPropO Σ).
+
+  Definition awkN : namespace := nroot .@ "awkN".
+  Definition awk_inv C i a :=
+    (∃ x:bool, sts_state_loc (A:=Addr) C i x
+            ∗ if x
+              then a ↦ₐ WInt 1%Z
+              else a ↦ₐ WInt 0%Z)%I.
+
+  Definition awk_rel_pub := λ a b, a = false ∨ b = true.
+  Definition awk_rel_priv := λ (a b : bool), True.
+
+  Lemma rtc_rel_pub y x :
+    y = (encode true) ->
+    rtc (convert_rel awk_rel_pub) y x ->
+    x = (encode true).
+  Proof.
+    intros Heq Hrtc.
+    induction Hrtc; auto.
+    rewrite Heq in H.
+    inversion H as [y' [b [Heq1 [Heq2 Hy] ] ] ].
+    inversion Hy; subst; auto.
+    apply encode_inj in Heq1. inversion Heq1.
+  Qed.
+  Lemma rtc_rel_pub' x :
+    rtc (convert_rel awk_rel_pub) (encode true) (encode x) ->
+    x = true.
+  Proof.
+    intros Hrtc.
+    apply encode_inj.
+    apply rtc_rel_pub with (encode true); auto.
+  Qed.
+
+  Lemma rtc_rel_pub_inv y x :
+    y = (encode true) ∨ y = (encode false) ->
+    rtc (convert_rel awk_rel_pub) y x ->
+    x = (encode true) ∨ x = (encode false).
+  Proof.
+    intros Heq Hrtc.
+    induction Hrtc; auto.
+    destruct Heq; subst.
+    + inversion H as [y' [b [Heq1 [Heq2 Hy] ] ] ]; simplify_eq.
+      apply IHHrtc. destruct b; auto.
+    + inversion H as [y' [b [Heq1 [Heq2 Hy] ] ] ]; simplify_eq.
+      apply IHHrtc. destruct b; auto.
+  Qed.
+
+  Lemma awk_rel_pub_inv (b : bool) (d d' : positive) :
+    d = encode b ->
+    rtc (convert_rel awk_rel_pub) d d' ->
+    ∃ b : bool, d' = encode b.
+  Proof.
+    intros Hd Hrtc.
+    assert (d' = encode true ∨ (d' = encode false)).
+    { eapply rtc_rel_pub_inv; last done.
+      destruct b ; auto.
+    }
+    destruct H; eexists; eauto.
+  Qed.
+
+  Lemma rtc_rel_inv y x :
+    y = (encode true) ∨ y = (encode false) ->
+    rtc (λ x y : positive,
+         convert_rel awk_rel_pub x y
+         ∨ convert_rel awk_rel_pub x y ∨ convert_rel awk_rel_priv x y) y x ->
+    x = (encode true) ∨ x = (encode false).
+  Proof.
+    intros Heq Hrtc.
+    induction Hrtc; auto.
+    destruct Heq; subst.
+    + destruct H as [ | [] ].
+      all: inversion H as [y' [b [Heq1 [Heq2 Hy] ] ] ]; simplify_eq.
+      all: apply IHHrtc; destruct b; auto.
+    + destruct H as [ | [] ].
+      all: inversion H as [y' [b [Heq1 [Heq2 Hy] ] ] ]; simplify_eq.
+      all: apply IHHrtc; destruct b; auto.
+  Qed.
+
+  Lemma awk_rel_inv (b : bool) (d d' : positive) :
+    d = encode b ->
+    rtc (λ x y : positive,
+         convert_rel awk_rel_pub x y
+         ∨ convert_rel awk_rel_pub x y ∨ convert_rel awk_rel_priv x y) d d' ->
+    ∃ b : bool, d' = encode b.
+  Proof.
+    intros Hd Hrtc.
+    assert (d' = encode true ∨ (d' = encode false)).
+    { eapply rtc_rel_inv; last done.
+      destruct b ; auto.
+    }
+    destruct H; eexists; eauto.
+  Qed.
+
+
+  Lemma related_pub_W0_Wfixed (W0 W3 W6 : WORLD) (csp_b csp_e : Addr) (l : list Addr) ( i : positive) :
+    let W1 := revoke W0 in
+    let W2 := <l[i:=false]l>W1 in
+    let W4 := revoke W3 in
+    let W5 := <l[i:=true]l>W4 in
+    let W7 := (revoke W6) in
+    (∀ a : finz MemNum, W0.1 !! a = Some Temporary ↔ a ∈ l ++ finz.seq_between csp_b csp_e) ->
+    related_sts_pub_world W2 W3 ->
+    related_sts_pub_world
+      (std_update_multiple W2 (finz.seq_between (csp_b ^+ 4)%a csp_e) Temporary) W3 ->
+    related_sts_pub_world W5 W6 ->
+    related_sts_pub_world
+      (std_update_multiple W5 (finz.seq_between (csp_b ^+ 4)%a csp_e) Temporary) W6 ->
+    Forall (λ a : finz MemNum, W6.1 !! a = Some Revoked) l ->
+    Forall (λ a : finz MemNum, W6.1 !! a = Some Revoked) (finz.seq_between csp_b (csp_b ^+ 4)%a) ->
+    finz.seq_between csp_b csp_e = finz.seq_between csp_b (csp_b ^+ 4)%a ++ finz.seq_between (csp_b ^+ 4)%a csp_e ->
+    wrel W6 !! i = Some (convert_rel awk_rel_pub, convert_rel awk_rel_pub, convert_rel awk_rel_priv) ->
+    loc W6 !! i = Some (encode true) ->
+    wrel W0 !! i = Some (convert_rel awk_rel_pub, convert_rel awk_rel_pub, convert_rel awk_rel_priv) ->
+    (exists b : bool, loc W0 !! i = Some (encode b)) ->
+
+    related_sts_pub_world W0
+      (close_list (l ++ finz.seq_between csp_b csp_e) W7).
+  Proof.
+    intros W1 W2 W4 W5 W7.
+    intros Htemporaries_W0 Hrelated_pub_W2_W3 Hrelated_pub_W2ext_W3 Hrelated_pub_W5_W6 Hrelated_pub_W5ext_W6
+      HW6_revoked_l Hrevoked_stk_l Hsplit_csp Hwrel_i Hwloc_i Hwrel_i_0 Hwloc_i_0.
+
+    assert ( related_sts_priv_world W0 W6 ) as Hrelated_priv_W0_W6.
+    { eapply (related_sts_priv_trans_world _ W3); eauto.
+      + eapply (related_sts_priv_pub_trans_world _ W2); eauto.
+        subst W2 W1.
+        eapply (related_sts_priv_trans_world _ (revoke W0)).
+        * apply revoke_related_sts_priv_world.
+        * destruct Hwloc_i_0 as [b Hwloc_i_0].
+          eapply related_sts_priv_world_loc_update; eauto.
+          right;right; apply convert_rel_of_rel; done.
+      + eapply (related_sts_priv_pub_trans_world _ W5); eauto.
+        subst W4 W5.
+        eapply (related_sts_priv_trans_world _ (revoke W3)).
+        * apply revoke_related_sts_priv_world.
+        *
+          destruct Hrelated_pub_W2_W3 as [HW2_W3_std (Hdom_loc_2_3 & Hdom_rel_2_3 & Hrtc_loc_2_3)].
+          assert (∃ d_W3, loc W3 !! i = Some d_W3) as [d_W3 Hd_W3].
+          { apply elem_of_dom.
+            apply Hdom_loc_2_3.
+            rewrite dom_insert.
+            rewrite elem_of_union; right.
+            apply elem_of_dom.
+            set_solver+Hwloc_i_0.
+          }
+          assert (∃ r1 r2 r3, wrel W3 !! i = Some (r1, r2, r3)) as (r1 & r2 & r3 & HW3_rel).
+          { assert (is_Some (wrel W0 !! i)) as HW0_rel_some by set_solver+Hwrel_i_0.
+            apply elem_of_dom in HW0_rel_some.
+            apply Hdom_rel_2_3 in HW0_rel_some.
+            apply elem_of_dom in HW0_rel_some as [ [ [] ] HW3_rel].
+            eexists _,_,_; eauto.
+          }
+          destruct Hwloc_i_0 as [b Hwloc_i_0].
+          specialize (Hrtc_loc_2_3 i _ _ _ _ _ _ Hwrel_i_0 HW3_rel) as (<- & <- & <- & Hrtc_loc_0_3).
+          ospecialize (Hrtc_loc_0_3 _ _ _ Hd_W3); first by simplify_map_eq.
+          eapply awk_rel_pub_inv in Hrtc_loc_0_3 as [b' ->]; last done.
+          eapply related_sts_priv_world_loc_update; eauto.
+          right;right; apply convert_rel_of_rel; done.
+    }
+    split; cbn; cycle 1.
+    - destruct W0 as [W0_std [W0_loc W0_rel] ],
+                 W3 as [W3_std [W3_loc W3_rel] ],
+                   W6 as [W6_std [W6_loc W6_rel] ]
+                   ; cbn.
+      destruct Hrelated_pub_W2_W3 as [HW2_W3_std HW2_W3_cus].
+      destruct Hrelated_pub_W5_W6 as [HW5_W6_std HW5_W6_cus].
+      destruct Hrelated_priv_W0_W6 as [HW0_W6_std HW0_W6_cus].
+      destruct HW0_W6_cus as (Hdom_loc_0_6 & Hdom_rel_0_6 & Hrtc_loc_0_6); cbn in *.
+      split;[|split];auto.
+      intros d r1 r2 r1' r2' r3 r3' HW0_rel HW6_rel.
+      specialize (Hrtc_loc_0_6 d _ _ _ _ _ _ HW0_rel HW6_rel) as (-> & -> & -> & Hrtc_loc_0_6).
+      repeat (split;first done).
+      intros d_W0 d_W6 Hd_W0 Hd_W6.
+      destruct HW2_W3_cus as (Hdom_loc_2_3 & Hdom_rel_2_3 & Hrtc_loc_2_3); cbn in *.
+      assert (∃ d_W3, W3_loc !! d = Some d_W3) as [d_W3 Hd_W3].
+      { apply elem_of_dom.
+        apply Hdom_loc_2_3.
+        rewrite dom_insert.
+        rewrite elem_of_union; right.
+        apply elem_of_dom.
+        set_solver+Hd_W0.
+      }
+      assert (∃ r1 r2 r3, W3_rel !! d = Some (r1, r2, r3)) as (r1 & r2 & r3 & HW3_rel).
+      { assert (is_Some (W0_rel !! d)) as HW0_rel_some by set_solver+HW0_rel.
+        apply elem_of_dom in HW0_rel_some.
+        apply Hdom_rel_2_3 in HW0_rel_some.
+        apply elem_of_dom in HW0_rel_some as [ [ [] ] HW3_rel].
+        eexists _,_,_; eauto.
+      }
+
+      destruct (decide (d = i)); simplify_eq.
+      + destruct Hwloc_i_0 as [b Hwloc_i_0]; simplify_eq.
+        apply rtc_once.
+        destruct HW5_W6_cus as (Hdom_loc_5_6 & Hdom_rel_5_6 & Hrtc_loc_5_6); cbn in *.
+        apply convert_rel_of_rel.
+        by right.
+      + eapply (rtc_transitive d_W0 d_W3 d_W6).
+        * specialize (Hrtc_loc_2_3 d _ _ _ _ _ _ HW0_rel HW3_rel) as (-> & -> & -> & Hrtc_loc_0_3).
+          ospecialize (Hrtc_loc_0_3 d_W0 d_W3 _ Hd_W3).
+          { by simplify_map_eq. }
+          done.
+        * destruct HW5_W6_cus as (Hdom_loc_5_6 & Hdom_rel_5_6 & Hrtc_loc_5_6); cbn in *.
+          specialize (Hrtc_loc_5_6 d _ _ _ _ _ _ HW3_rel HW6_rel) as (-> & -> & -> & Hrtc_loc_5_6).
+          ospecialize (Hrtc_loc_5_6 d_W3 d_W6 _ Hd_W6).
+          { by simplify_map_eq. }
+          done.
+    - cbn in *.
+      split.
+      {
+        intros a Ha.
+        rewrite elem_of_dom -close_list_std_sta_is_Some -revoke_std_sta_lookup_Some -elem_of_dom.
+        destruct Hrelated_pub_W5_W6 as [ [Hdom_W5_W6 _] _].
+        apply Hdom_W5_W6.
+        rewrite -revoke_dom_eq.
+        destruct Hrelated_pub_W2_W3 as [ [Hdom_W2_W3 _] _].
+        apply Hdom_W2_W3.
+        by rewrite -revoke_dom_eq.
+      }
+      intros a ρ0 ρ2 Ha0 Ha2.
+      destruct ρ0; cycle 1.
+      + (* the initial a was in the Permanent state *)
+        assert (a ∉ l ++ finz.seq_between csp_b csp_e) as Ha_notin.
+        { destruct (Htemporaries_W0 a) as [_ ?].
+          intro Hcontra; apply H in Hcontra. by rewrite Ha0 in Hcontra.
+        }
+        apply revoke_lookup_Perm in Ha0.
+        assert (std W3 !! a = Some Permanent) as Ha0_W3.
+        { rewrite (region_state_pub_perm W2); eauto. }
+        assert (std W6 !! a = Some Permanent) as Ha0_W6.
+        { rewrite (region_state_pub_perm W5); eauto.
+          subst W5. cbn.
+          rewrite revoke_lookup_Perm; eauto.
+        }
+        rewrite -close_list_std_sta_same in Ha2; eauto.
+        apply revoke_lookup_Perm in Ha0_W6.
+        simplify_map_eq.
+        apply rtc_refl.
+      + (* the initial a was in the Revoked state *)
+        destruct ρ2; last apply rtc_refl; apply rtc_once; constructor.
+      + (* the initial a was in the Temporary state *)
+        assert (a ∈ l ++ finz.seq_between csp_b csp_e) as Ha_in.
+        { destruct (Htemporaries_W0 a) as [? _]; by apply Htemporaries_W0. }
+        apply revoke_lookup_Monotemp in Ha0.
+        assert (std W1 !! a = Some Revoked) as Ha0_W1.
+        { done. }
+        assert (std W2 !! a = Some Revoked) as Ha0_W2.
+        { done. }
+        assert (
+            std ((std_update_multiple W2 (finz.seq_between (csp_b ^+ 4)%a csp_e)
+                    Temporary)) !! a =
+            Some (if (decide (a ∈ (finz.seq_between (csp_b ^+ 4)%a csp_e)))
+                  then Temporary
+                  else Revoked
+          )).
+        {
+          destruct (decide (a ∈ (finz.seq_between (csp_b ^+ 4)%a csp_e))) as [Ha_in_stk | Ha_in_stk].
+          + apply std_sta_update_multiple_lookup_in_i; eauto.
+          + rewrite std_sta_update_multiple_lookup_same_i; eauto.
+        }
+
+        destruct (decide (a ∈ finz.seq_between (csp_b ^+ 4)%a csp_e)) as [Ha_in''|Ha_in''].
+        * assert (std W3 !! a = Some Temporary) as Ha0_W3.
+          { eapply region_state_pub_temp; eauto. }
+          assert (std W4 !! a = Some Revoked) as Ha0_W4.
+          { by apply revoke_lookup_Monotemp. }
+          assert (std W5 !! a = Some Revoked) as Ha0_W5 by done.
+          assert (
+              std (std_update_multiple W5 (finz.seq_between (csp_b ^+ 4)%a csp_e) Temporary) !! a = Some Temporary
+            ) as Ha0_W5ext.
+          { apply std_sta_update_multiple_lookup_in_i; eauto. }
+          assert (std W6 !! a = Some Temporary) as Ha0_W6.
+          { eapply region_state_pub_temp; eauto. }
+          assert (std W7 !! a = Some Revoked) as Ha0_W7.
+          { by apply revoke_lookup_Monotemp. }
+          eapply (close_list_std_sta_revoked _ _ _  Ha_in) in Ha0_W7; eauto.
+          rewrite Ha2 in Ha0_W7; simplify_eq.
+          apply rtc_refl.
+        * destruct (decide (a ∈ finz.seq_between csp_b (csp_b ^+ 4)%a)) as [Ha_in_save|Ha_in_save].
+          ** rewrite Forall_forall in Hrevoked_stk_l.
+             apply Hrevoked_stk_l in Ha_in_save.
+             apply revoke_lookup_Revoked in Ha_in_save.
+             eapply (close_list_std_sta_revoked _ _ _  Ha_in) in Ha_in_save; eauto.
+             rewrite Ha2 in Ha_in_save; simplify_eq.
+             apply rtc_refl.
+          ** assert (a ∈ l) as Ha_in_l.
+             { rewrite Hsplit_csp in Ha_in.
+               rewrite elem_of_app in Ha_in.
+               destruct Ha_in; first done.
+               rewrite elem_of_app in H0.
+               destruct H0; contradiction.
+             }
+             rewrite Forall_forall in HW6_revoked_l.
+             apply HW6_revoked_l in Ha_in_l.
+             apply revoke_lookup_Revoked in Ha_in_l.
+             eapply (close_list_std_sta_revoked _ _ _  Ha_in) in Ha_in_l; eauto.
+             rewrite Ha2 in Ha_in_l; simplify_eq.
+             apply rtc_refl.
+  Qed.
+
+End VAE_helper.
